icing/icing_optimisationsScript.sml
@@ -12,6 +12,10 @@ open preamble;
 
 val _ = new_theory "icing_optimisations";
 
+Definition reverse_tuple_def:
+  reverse_tuple (a, b) = (b, a)
+End
+
 (*
   Generator for commutativity rewrites
 *)
@@ -45,6 +49,20 @@ val fp_mul_assoc_def =
   curry save_thm "fp_mul_assoc_def"
     (Q.SPEC `FP_Mul` fp_assoc_gen_def);
 
+Definition fp_assoc2_gen_def:
+  fp_assoc2_gen op = reverse_tuple (fp_assoc_gen op)
+End
+
+(* Associativity of + *)
+val fp_add_assoc2_def =
+  curry save_thm "fp_add_assoc2_def"
+    (Q.SPEC `FP_Add` fp_assoc2_gen_def);
+
+(* Associativity of * *)
+val fp_mul_assoc2_def =
+  curry save_thm "fp_mul_assoc2_def"
+    (Q.SPEC `FP_Mul` fp_assoc2_gen_def);
+
 (*
   FMA introudction
 *)
@@ -53,10 +71,23 @@ Definition fp_fma_intro_def:
                   Terop FP_Fma (Var 2) (Var 0) (Var 1))
 End
 
-(* Subtraction -> Addtion of inverse *)
+(* Subtraction -> Addition of inverse *)
 Definition fp_sub_add_def:
   fp_sub_add = (Binop FP_Sub (Var 0) (Var 1),
                 Binop FP_Add (Var 0) (Unop FP_Neg (Var 1)))
+End
+
+Definition fp_add_sub_def:
+  fp_add_sub = reverse_tuple fp_sub_add
+End
+
+Definition fp_times_minus_one_neg_def:
+  (* 13830554455654793216 is -1.0 in binary representation *)
+  fp_times_minus_one_neg = (Binop FP_Mul (Var 0) (Word (13830554455654793216w: word64)), Unop FP_Neg (Var 0))
+End
+
+Definition fp_neg_times_minus_one_def:
+  fp_neg_times_minus_one = reverse_tuple fp_times_minus_one_neg
 End
 
 (* Unary - can be pushed into multiplications; this matches a addition above,
@@ -66,5 +97,97 @@ Definition fp_neg_push_mul_r_def:
   (Binop FP_Add (Unop FP_Neg (Binop FP_Mul (Var 0) (Var 1))) (Var 2),
    Binop FP_Add (Binop FP_Mul (Var 0) (Unop FP_Neg (Var 1))) (Var 2))
 End
+
+Definition fp_times_two_to_add_def:
+  (* 2.0 is 4611686018427387904 in binary representation *)
+  fp_times_two_to_add = (Binop FP_Mul (Var 0) (Word (4611686018427387904w: word64)),
+                         Binop FP_Add (Var 0) (Var 0))
+End
+
+Definition fp_times_three_to_add_def:
+  (* 3.0 is 4613937818241073152 in binary representation *)
+  fp_times_three_to_add = (Binop FP_Mul (Var 0) (Word (4613937818241073152w: word64)),
+                           Binop FP_Add (Binop FP_Add (Var 0) (Var 0)) (Var 0))
+End
+
+Definition fp_times_zero_def:
+  fp_times_zero = (Binop FP_Mul (Var 0) (Word (0w: word64)), Word (0w: word64))
+End
+
+Definition fp_plus_zero_def:
+  fp_plus_zero = (Binop FP_Add (Var 0) (Word (0w: word64)), (Var 0))
+End
+
+Definition fp_times_one_def:
+  (* 4607182418800017408 is 1.0 in binary representation *)
+  fp_times_one = (Binop FP_Mul (Var 0) (Word (4607182418800017408w: word64)), (Var 0))
+End
+
+Definition fp_times_one_reverse_def:
+  (* 4607182418800017408 is 1.0 in binary representation *)
+  fp_times_one_reverse = reverse_tuple fp_times_one
+End
+
+Definition fp_times_into_div_def:
+  fp_times_into_div = (Binop FP_Mul (Binop FP_Div (Var 0) (Var 1)) (Var 2), Binop FP_Div (Binop FP_Mul (Var 0) (Var 2)) (Var 1))
+End
+
+Definition fp_same_sub_def:
+  fp_same_sub = (Binop FP_Sub (Var 0) (Var 0), (Word (0w: word64)))
+End
+
+Definition fp_same_div_def:
+  (* 4607182418800017408 is 1.0 in binary representation *)
+  fp_same_div = (Binop FP_Div (Var 0) (Var 0), (Word (4607182418800017408w: word64)))
+End
+
+Definition fp_distribute_gen_def:
+  fp_distribute_gen opInner opOuter = (Binop opOuter (Binop opInner (Var 0) (Var 2)) (Binop opInner (Var 1) (Var 2)),
+                                       Binop opInner (Binop opOuter (Var 0) (Var 1)) (Var 2))
+End
+
+(* Distributivity of * and + *)
+val fp_mul_add_distribute_def =
+  curry save_thm "fp_mul_add_distribute_def"
+    (Q.SPECL [‘FP_Mul’, ‘FP_Add’] fp_distribute_gen_def);
+
+(* Distributivity of * and - *)
+val fp_mul_sub_distribute_def =
+  curry save_thm "fp_mul_sub_distribute_def"
+    (Q.SPECL [‘FP_Mul’, ‘FP_Sub’] fp_distribute_gen_def);
+
+(* Distributivity of / and + *)
+val fp_div_add_distribute_def =
+  curry save_thm "fp_div_add_distribute_def"
+    (Q.SPECL [‘FP_Div’, ‘FP_Add’] fp_distribute_gen_def);
+
+(* Distributivity of / and - *)
+val fp_div_sub_distribute_def =
+  curry save_thm "fp_div_sub_distribute_def"
+    (Q.SPECL [‘FP_Div’, ‘FP_Sub’] fp_distribute_gen_def);
+
+Definition fp_undistribute_gen_def:
+  fp_undistribute_gen opInner opOuter = reverse_tuple (fp_distribute_gen opInner opOuter)
+End
+
+(* Reverse Distributivity of * and + *)
+val fp_mul_add_undistribute_def =
+  curry save_thm "fp_mul_add_undistribute_def"
+    (Q.SPECL [‘FP_Mul’, ‘FP_Add’] fp_undistribute_gen_def);
+
+(* Reverse Distributivity of * and - *)
+val fp_mul_sub_undistribute_def =
+  curry save_thm "fp_mul_sub_undistribute_def"
+    (Q.SPECL [‘FP_Mul’, ‘FP_Sub’] fp_undistribute_gen_def);
+
+(* Reverse Distributivity of / and + *)
+val fp_div_add_undistribute_def =
+  curry save_thm "fp_div_add_undistribute_def"
+    (Q.SPECL [‘FP_Div’, ‘FP_Add’] fp_undistribute_gen_def);
+
+(* Reverse Distributivity of / and - *)
+val fp_div_sub_undistribute_def =
+  curry save_thm "fp_div_sub_undistribute_def"
+    (Q.SPECL [‘FP_Div’, ‘FP_Sub’] fp_undistribute_gen_def);
 
 val _ = export_theory ();
